cogent/examples/wa_connect/WordArray_UpdCCorres.thy
@@ -102,36 +102,39 @@ lemma upd_C_wordarray_put2_corres:
    apply (erule_tac x = "t2_C.idx_C v'" in allE)+
    apply (clarsimp simp: val_rel_simp heap_simp type_rel_simp)
   apply clarsimp
-  apply (rule_tac x = "\<lambda>l. (if l = arr + 4 * t2_C.idx_C v' \<and> t2_C.idx_C v' < len 
-                            then option.Some (UPrim (LU32 (t2_C.val_C v'))) 
-                            else \<sigma> l)" in exI)
-  apply (rule_tac x = "UPtr (ptr_val y') (RCon ''WordArray'' [RPrim (Num U32)])" in exI)
+  apply (monad_eq simp: upd_wa_put2_0_def \<xi>0.simps)
+  apply (case_tac "idx_C v' < len"; clarsimp)
   apply (rule conjI)
-   apply (monad_eq simp: wordarray_put2_0'_def upd_wa_put2_0_def \<xi>0.simps)
-  apply (rule conjI)
-   apply (rule_tac x = "RCon ''WordArray'' [RPrim (Num U32)]" in exI, simp)
-  apply (clarsimp simp: state_rel_def heap_rel_def heap_rel_ptr_meta heap_rel_ptr_w32_meta)
-  apply (rule conjI)
-   apply (clarsimp simp: heap_rel_meta_def)
-   apply (rule conjI; clarsimp)
-    apply (clarsimp simp: type_rel_simp)
+    apply (monad_eq simp: wordarray_put2_0'_def)
+   apply (clarsimp simp: state_rel_def heap_rel_def heap_rel_ptr_meta heap_rel_ptr_w32_meta)
    apply (monad_eq simp: wordarray_put2_0'_def)
-   apply (case_tac "idx_C v' < SCAST(32 signed \<rightarrow> 32) (len_C (heap_WordArray_u32_C st (t2_C.arr_C v')))"; 
-          drule_tac p = x and uv = uv in all_heap_rel_ptrD; clarsimp simp: is_valid_simp heap_simp)
-  apply (erule_tac x = "t2_C.arr_C v'" in allE)
-  apply (clarsimp simp: heap_rel_meta_def wa_abs_repr_def type_rel_simp val_rel_simp)
-  apply (monad_eq simp: wordarray_put2_0'_def heap_simp is_valid_simp)
-  apply (rule conjI; clarsimp)
-   apply (drule_tac p = "values_C (heap_WordArray_u32_C st (t2_C.arr_C v')) +\<^sub>p uint (t2_C.idx_C v')" and 
-                   uv = uv in all_heap_rel_ptrD; clarsimp simp: type_rel_simp val_rel_simp)
-  apply (rule conjI)
+   apply (frule_tac p = "t2_C.arr_C v'" in all_heap_rel_ptrD; simp?)
+    apply (clarsimp simp: type_rel_simp wa_abs_repr_def)
+   apply (clarsimp simp: val_rel_simp heap_simp is_valid_simp)
+   apply (drule wa_abs_typing_u_elims(5))
+   apply (erule_tac x = "t2_C.idx_C v'" in allE; clarsimp)
+   apply (drule_tac upd_h = "(heap_w32_update 
+      (\<lambda>x. x(values_C (heap_WordArray_u32_C st (t2_C.arr_C v')) +\<^sub>p uint (idx_C v') := val_C v')) st)" and
+      x = "(values_C (heap_WordArray_u32_C st (t2_C.arr_C v'))) +\<^sub>p uint (idx_C v')" and
+      uv' = "UPrim (LU32 (val_C v'))" and uv = "UPrim x"
+      in all_heap_rel_updE; simp?; clarsimp?)
+    apply (clarsimp simp: type_rel_simp)
+   apply (drule_tac upd_h = "(heap_w32_update
+      (\<lambda>x. x(values_C (heap_WordArray_u32_C st (t2_C.arr_C v')) +\<^sub>p uint (idx_C v') := val_C v')) st)" and
+      x = "(values_C (heap_WordArray_u32_C st (t2_C.arr_C v'))) +\<^sub>p uint (idx_C v')" and
+      uv' = "UPrim (LU32 (val_C v'))" and uv = "UPrim x"
+      in all_heap_rel_updE; simp?; clarsimp?)
+   apply (rule conjI, clarsimp simp: val_rel_simp)
+   apply clarsimp
+   apply (rule FalseE)
+   apply (cut_tac p = p and q = "((values_C (heap_WordArray_u32_C st (t2_C.arr_C v'))) +\<^sub>p uint (idx_C v'))" in ptr_val_inj)
    apply (clarsimp simp: ptr_add_def)
-   apply (metis Ptr_ptr_val mult.commute)
-  apply clarsimp
-  apply (case_tac "idx_C v' < SCAST(32 signed \<rightarrow> 32) (len_C (heap_WordArray_u32_C st (t2_C.arr_C v')))";
-         drule_tac p = x and uv = uv in all_heap_rel_ptrD; clarsimp simp: type_rel_simp val_rel_simp)
+  apply (monad_eq simp: wordarray_put2_0'_def)
+  apply (clarsimp simp: state_rel_def heap_rel_def heap_rel_ptr_meta)
+  apply (frule_tac p = "t2_C.arr_C v'" in all_heap_rel_ptrD; simp?)
+   apply (clarsimp simp: type_rel_simp wa_abs_repr_def)
+  apply (clarsimp simp: val_rel_simp heap_simp is_valid_simp)
   done
-
 
 lemma upd_C_wordarray_length_corres:
 "\<And>i \<gamma> v' \<Gamma>' \<sigma> st.
@@ -836,13 +839,17 @@ lemma
    apply (rule corres_mul; simp)
   apply (clarsimp simp: \<Xi>_def wordarray_fold_no_break_0_type_def mul_type_def abbreviated_type_defs)
   done
-thm validNF_def valid_def no_fail_def
+
+lemma \<Xi>_wordarray_fold_no_break_0:
+  "\<Xi> ''wordarray_fold_no_break_0'' = wordarray_fold_no_break_0_type"
+  by (clarsimp simp: \<Xi>_def)
 
 lemma fold_dispatch_wp:
   "\<lbrakk>proc_ctx_wellformed \<Xi>; upd.proc_env_matches_ptrs \<xi>0 \<Xi>;
     wa_abs_typing_u (UWA (TPrim (Num U32)) len arr) ''WordArray'' [TPrim (Num U32)] (Boxed ReadOnly ptrl) r w \<sigma>;
     \<sigma> p = option.Some (UAbstract (UWA (TPrim (Num U32)) len arr));
-    upd.uval_typing \<Xi> \<sigma> acc (TPrim (Num U32)) ra wa; upd.uval_typing \<Xi> \<sigma> obsv TUnit ro {};
+    upd.uval_typing \<Xi> \<sigma> acc (foldmap_acc_type ''wordarray_fold_no_break_0'') ra wa;
+    upd.uval_typing \<Xi> \<sigma> obsv (foldmap_obsv_type ''wordarray_fold_no_break_0'') ro {};
     wa \<inter> r = {}; wa \<inter> ro = {}; p \<notin> wa;
     (\<Xi>, [], [option.Some (foldmap_funarg_type ''wordarray_fold_no_break_0'')] \<turnstile> 
     (App f (Var 0)) : (foldmap_funret_type ''wordarray_fold_no_break_0''));
@@ -861,11 +868,7 @@ lemma fold_dispatch_wp:
       foldmap_inv_stat obsv (t3_C.obsv_C args) \<and> foldmap_bounds frm to len (n + 1) e \<and> 
       foldmap_measure (n + 1) to < foldmap_measure n' to\<rbrace>!"
   apply (subst validNF_def)
-  apply (clarsimp simp: \<Xi>_def wordarray_fold_no_break_0_type_def abbreviated_type_defs)
-  apply (subst (asm) abbreviated_type_defs[symmetric])+
-  apply (subst (asm) wordarray_fold_no_break_0_type_def[symmetric])+
-  apply (subst (asm) \<Xi>_def[symmetric])+
-  apply (clarsimp simp: abbreviated_type_defs)
+  apply (clarsimp simp: \<Xi>_wordarray_fold_no_break_0 wordarray_fold_no_break_0_type_def abbreviated_type_defs)
   apply (rule conjI)
    apply (subst valid_def)
    apply (clarsimp simp: foldmap_inv_def)
@@ -877,13 +880,12 @@ lemma fold_dispatch_wp:
     apply (subst val_rel_simp; simp add: foldmap_inv_stat_def)
    apply (erule_tac x = \<sigma>' in allE)
    apply (erule_tac x = sa in allE)
-   apply (clarsimp simp: corres_def val_rel_simp)
+   apply (clarsimp simp: corres_def)
    apply (frule_tac t = "TPrim (Num U32)" in upd_wa_foldnb_bod_preservation[rotated 2]; simp?; clarsimp?)
    apply (rename_tac r' w')
-   apply (subgoal_tac "upd.matches_ptrs \<Xi> \<sigma>' [URecord [(UPrim (LU32 v), RPrim (Num U32)),
-      (UPrim (LU32 (t3_C.acc_C a)), RPrim (Num U32)), (obsv, upd.uval_repr obsv)]]
-      [option.Some (TRecord [(''elem'', TPrim (Num U32), Present), (''acc'', TPrim (Num U32), Present),
-        (''obsv'', TUnit, Present)] Unboxed)] (r' \<union> ro) w'")
+   apply (subgoal_tac "upd.matches_ptrs \<Xi> \<sigma>' [(mk_urecord [x, res, obsv])]
+      [option.Some (foldmap_funarg_type ''wordarray_fold_no_break_0'')] (r' \<union> ro) w'")
+    apply (clarsimp simp: \<Xi>_wordarray_fold_no_break_0 wordarray_fold_no_break_0_type_def abbreviated_type_defs)
     apply (erule impE, blast)
     apply clarsimp
     apply (erule_tac x = ret in allE)
@@ -891,7 +893,7 @@ lemma fold_dispatch_wp:
     apply clarsimp
     apply (drule upd.preservation[where \<tau>s = "[]" and K = "[]", simplified]; simp?)
     apply clarsimp
-    apply (rename_tac \<sigma>'' rb wb)
+    apply (rename_tac \<sigma>'' res' rb wb)
     apply (clarsimp simp: foldmap_bounds_def)
     apply (case_tac "frm < to \<and> frm < len"; clarsimp)
     apply (frule wa_abs_typing_u_elims(5))
@@ -901,7 +903,7 @@ lemma fold_dispatch_wp:
      apply (drule_tac t = U32 in  wa_abs_typing_u_elims(2)[where \<tau>s = "[_]", simplified]; simp)
      apply blast
     apply clarsimp
-    apply (drule_tac t = U32 and arr = arr and len = len and r' = "UPrim (LU32 ret)" 
+    apply (drule_tac t = U32 and arr = arr and len = len and r' = res' 
       in upd_wa_foldnb_bod_step; simp?; clarsimp?)
      apply (rule conjI)
       apply (drule_tac p = p in readonly_not_in_frame; simp?)
@@ -927,25 +929,30 @@ lemma fold_dispatch_wp:
      apply (drule wa_abs_typing_u_elims(2); clarsimp)
      apply blast
     apply (rule conjI)
-     apply (rule_tac x = \<sigma>'' in exI; simp)
+     apply (rule_tac x = \<sigma>'' in exI)
+     apply (rule_tac x = res' in exI; simp)
     apply (frule_tac a = n and k = to in less_is_non_zero_p1)
     apply (drule unatSuc2; clarsimp simp: word_less_nat_alt word_le_nat_alt foldmap_measure_def)
     apply linarith
+   apply (clarsimp simp: \<Xi>_wordarray_fold_no_break_0 wordarray_fold_no_break_0_type_def abbreviated_type_defs)
    apply (rule upd.matches_ptrs_some[where r' = "{}" and w' = "{}", simplified])
     apply (rule upd.u_t_struct; simp?)
     apply (rule upd.u_t_r_cons1[where r = "{}" and w = "{}", simplified]; simp?)
-     apply (rule upd.u_t_prim'; clarsimp)
-    apply (rule upd.u_t_r_cons1[where r' = ro and w' = "{}", simplified]; simp?)
-     apply (drule_tac u = obsv in upd.uval_typing_frame(1); simp?)
-      apply blast
-     apply (rule upd.u_t_r_cons1[where r' = "{}" and w' = "{}", simplified]; simp?)
-      apply (rule upd.u_t_r_empty)
-     apply (erule u_t_unittE; clarsimp)
-    apply (rule disjointI)
-    apply (frule_tac p = y and r = ro in upd.uval_typing_valid(1)[where w = "{}", simplified]; simp?)
-    apply clarsimp
-    apply (drule_tac p = y in readonly_not_in_frame; simp?)
-    apply (drule_tac x = y and S' = ro in orthD2; simp?)
+      apply (subst (asm) val_rel_word; clarsimp)
+      apply (rule upd.u_t_prim'; clarsimp)
+     apply (rule upd.u_t_r_cons1[where r' = ro and w' = "{}", simplified]; simp?)
+       apply (drule_tac u = obsv in upd.uval_typing_frame(1); simp?)
+        apply blast
+       apply (rule upd.u_t_r_cons1[where r' = "{}" and w' = "{}", simplified]; simp?)
+        apply (rule upd.u_t_r_empty)
+       apply (drule_tac v = obsv in upd.type_repr_uval_repr(1); simp)
+      apply (rule disjointI)
+      apply (frule_tac p = y and r = ro in upd.uval_typing_valid(1)[where w = "{}", simplified]; simp?)
+      apply clarsimp
+      apply (drule_tac p = y in readonly_not_in_frame; simp?)
+      apply (drule_tac x = y and S' = ro in orthD2; simp?)
+     apply (drule_tac v = res in upd.type_repr_uval_repr(1); simp)
+    apply (subst (asm) val_rel_word; clarsimp)
    apply (rule upd.matches_ptrs_empty[where \<tau>s = "[]", simplified])
   apply (subst no_fail_def)
   apply clarsimp
@@ -958,7 +965,7 @@ lemma fold_dispatch_wp:
    apply (subst val_rel_simp; simp add: foldmap_inv_stat_def)
   apply (erule_tac x = \<sigma>' in allE)
   apply (erule_tac x = sa in allE)
-  apply (clarsimp simp: corres_def val_rel_simp)
+  apply (clarsimp simp: corres_def)
   apply (frule_tac t = "TPrim (Num U32)" in upd_wa_foldnb_bod_preservation[rotated 2]; simp?; clarsimp?)
   apply (rename_tac r' w')
   apply (erule_tac x = "r' \<union> ro" in allE)
@@ -968,28 +975,33 @@ lemma fold_dispatch_wp:
   apply (rule upd.matches_ptrs_some[where r' = "{}" and w' = "{}", simplified])
    apply (rule upd.u_t_struct; simp?)
    apply (rule upd.u_t_r_cons1[where r = "{}" and w = "{}", simplified]; simp?)
-    apply (rule upd.u_t_prim'; clarsimp)
-   apply (rule upd.u_t_r_cons1[where r' = ro and w' = "{}", simplified]; simp?)
-    apply (drule_tac u = obsv in upd.uval_typing_frame(1); simp?)
-     apply blast
-    apply (rule upd.u_t_r_cons1[where r' = "{}" and w' = "{}", simplified]; simp?)
-     apply (rule upd.u_t_r_empty)
-    apply (erule u_t_unittE; clarsimp)
-   apply (rule disjointI)
-   apply (frule_tac p = y and r = ro in upd.uval_typing_valid(1)[where w = "{}", simplified]; simp?)
-   apply clarsimp
-   apply (drule_tac p = y in readonly_not_in_frame; simp?)
-   apply (drule_tac x = y and S' = ro in orthD2; simp?)
+     apply (subst (asm) val_rel_word; clarsimp)
+     apply (rule upd.u_t_prim'; clarsimp)
+    apply (rule upd.u_t_r_cons1[where r' = ro and w' = "{}", simplified]; simp?)
+      apply (drule_tac u = obsv in upd.uval_typing_frame(1); simp?)
+       apply blast
+      apply (rule upd.u_t_r_cons1[where r' = "{}" and w' = "{}", simplified]; simp?)
+       apply (rule upd.u_t_r_empty)
+      apply (drule_tac v = obsv in upd.type_repr_uval_repr(1); simp)
+     apply (rule disjointI)
+     apply (frule_tac p = y and r = ro in upd.uval_typing_valid(1)[where w = "{}", simplified]; simp?)
+     apply clarsimp
+     apply (drule_tac p = y in readonly_not_in_frame; simp?)
+     apply (drule_tac x = y and S' = ro in orthD2; simp?)
+    apply (drule_tac v = res in upd.type_repr_uval_repr(1); simp)
+   apply (subst (asm) val_rel_word; clarsimp)
   apply (rule upd.matches_ptrs_empty[where \<tau>s = "[]", simplified])
   done
 
 
 lemma upd_C_wordarray_fold_no_break_corres':
-  "\<lbrakk>i < length \<gamma>; val_rel (\<gamma> ! i) v'; \<Gamma>' ! i = option.Some (prod.fst (prod.snd (\<Xi> ''wordarray_fold_no_break_0'')));
-   \<gamma> ! i = URecord fs; f = prod.fst (fs ! 3); upd.proc_env_matches_ptrs \<xi>0 \<Xi>;
-  (\<Xi>, [], [option.Some (foldmap_funarg_type ''wordarray_fold_no_break_0'')] \<turnstile> 
+  "\<lbrakk>upd.proc_env_matches_ptrs \<xi>0 \<Xi>; i < length \<gamma>; val_rel (\<gamma> ! i) v'; 
+    \<Gamma>' ! i = option.Some (prod.fst (prod.snd (\<Xi> ''wordarray_fold_no_break_0'')));
+    \<gamma> ! i = URecord fs; f = prod.fst (fs ! 3); obsv = prod.fst (fs ! 5);
+    upd.uval_typing \<Xi> \<sigma> obsv (foldmap_obsv_type ''wordarray_fold_no_break_0'') ro {};
+    (\<Xi>, [], [option.Some (foldmap_funarg_type ''wordarray_fold_no_break_0'')] \<turnstile> 
     (App (uvalfun_to_exprfun f) (Var 0)) : (foldmap_funret_type ''wordarray_fold_no_break_0''));
-   \<forall>x x' \<sigma> s. val_rel x x' \<longrightarrow> update_sem_init.corres wa_abs_typing_u wa_abs_repr (Generated.state_rel wa_abs_repr) 
+    \<forall>x x' \<sigma> s. val_rel x x' \<longrightarrow> update_sem_init.corres wa_abs_typing_u wa_abs_repr (Generated.state_rel wa_abs_repr) 
       (App (uvalfun_to_exprfun f) (Var 0)) (do ret <- dispatch_t4' (t5_C.f_C v') x'; gets (\<lambda>s. ret) od) 
       \<xi>0 [x] \<Xi> [option.Some (foldmap_funarg_type ''wordarray_fold_no_break_0'')] \<sigma> s\<rbrakk>
     \<Longrightarrow> update_sem_init.corres wa_abs_typing_u wa_abs_repr (Generated.state_rel wa_abs_repr)
@@ -1007,10 +1019,9 @@ gets (\<lambda>s. x)
   apply (subst (asm) val_rel_word)
   apply (subst (asm) val_rel_word)
   apply (clarsimp simp: upd_wa_foldnb_def wordarray_fold_no_break_0'_def)
-  apply (rename_tac pwa_rep frm_rep to_rep f_rep acc a_rep obsv o_rep wa_rep)
+  apply (rename_tac pwa_rep frm_rep to_rep f_rep acc a_rep o_rep wa_rep)
   apply (erule upd.u_t_recE; clarsimp)
-  apply (rotate_tac -3)
-  apply (subst (asm) \<Xi>_def; clarsimp simp: wordarray_fold_no_break_0_type_def abbreviated_type_defs)
+  apply (clarsimp simp: \<Xi>_wordarray_fold_no_break_0 wordarray_fold_no_break_0_type_def abbreviated_type_defs)
   apply (erule upd.u_t_r_consE; clarsimp)
   apply (erule upd.u_t_p_absE; clarsimp)
   apply (frule wa_abs_typing_u_elims(1); clarsimp)
@@ -1027,7 +1038,9 @@ gets (\<lambda>s. x)
   apply (frule upd.tfun_no_pointers(1))
   apply (frule upd.tfun_no_pointers(2))
   apply clarsimp
-  apply (rename_tac acc ra wa obsv ro wo)
+  apply (rename_tac acc ra wa ro' wo)
+  apply (drule_tac x = obsv in upd.uval_typing_unique_ptrs(1); simp?)
+  apply clarsimp
   apply (subst unknown_bind_ignore)+
   apply (clarsimp simp: join_guards)
   apply wp
@@ -1039,15 +1052,10 @@ gets (\<lambda>s. x)
           foldmap_inv_stat obsv (t3_C.obsv_C a) \<and>
           foldmap_bounds (t5_C.frm_C v') (t5_C.to_C v') len b e" in whileLoop_add_invI; simp?)
       apply (wp; clarsimp simp: unknown_bind_ignore split: prod.splits)
-          apply (rename_tac sa a n args a' n') thm fold_dispatch_wp
+          apply (rename_tac sa a n args a' n')
           apply (rule_tac a = a and wa = wa and ra = ra and ro = ro and w = "{}" and r = r and
             ptrl = undefined in fold_dispatch_wp[rotated 2]; simp?)
-             apply (subst (asm) upd.uval_typing.simps[of _ _ _ TUnit, simplified]; simp?)
-             apply (erule disjE; clarsimp?)+
-             apply (rule upd.u_t_unit)
-            apply (clarsimp simp: Int_Un_distrib2)
-           apply (clarsimp simp: \<Xi>_def wordarray_fold_no_break_0_type_def abbreviated_type_defs)
-          apply (clarsimp simp: \<Xi>_def wordarray_fold_no_break_0_type_def abbreviated_type_defs)
+             apply (clarsimp simp: \<Xi>_wordarray_fold_no_break_0 wordarray_fold_no_break_0_type_def abbreviated_type_defs)+
          apply wp
         apply wp
        apply clarsimp
@@ -1057,10 +1065,8 @@ gets (\<lambda>s. x)
        apply (erule_tac x = j in allE; clarsimp)
        apply (drule_tac acc = acc and obsv = obsv and rb = ra and wb = wa and rc = ro
           in upd_wa_foldnb_bod_preservation; simp?; clarsimp?)
-        apply (erule u_t_unittE; clarsimp intro!: upd.u_t_unit)
        apply (frule_tac p = "ptr_val (t5_C.arr_C v')" in valid_ptr_not_in_frame_same; simp?)
        apply (drule_tac p = "arr + 4 * j" in valid_ptr_not_in_frame_same; simp?)
-        apply (subst (asm) Int_Un_distrib2; clarsimp)
         apply (drule_tac x = "arr + 4 * j" and S = wa and S' = r in orthD2; simp?)
         apply (drule wa_abs_typing_u_elims(2); clarsimp)
         apply blast
@@ -1088,7 +1094,7 @@ gets (\<lambda>s. x)
       apply (rule conjI)
        apply (erule u_t_primtE; clarsimp)
       apply (rule conjI)
-       apply (erule u_t_unittE; clarsimp)
+       apply (drule_tac v = obsv in upd.type_repr_uval_repr(1); simp?)
       apply (rule conjI)
        apply (drule wa_abs_typing_u_elims(5); simp)
       apply (rule conjI)
@@ -1097,18 +1103,17 @@ gets (\<lambda>s. x)
       apply (rule_tac x = \<sigma>' in exI)
       apply (rule_tac x = res in exI)
       apply (clarsimp simp: foldmap_inv_def)
-      apply (rule_tac x = "TPrim (Num U32)" in exI)
-      apply (rule_tac x = TUnit in exI)
+      apply (rule_tac x = "foldmap_acc_type ''wordarray_fold_no_break_0''" in exI)
+      apply (rule_tac x = "foldmap_obsv_type ''wordarray_fold_no_break_0''" in exI)
       apply (rule_tac x = "''elem''" in exI)
       apply (rule_tac x = "''acc''" in exI)
       apply (rule_tac x = "''obsv''" in exI)
-      apply clarsimp
+      apply (clarsimp simp: \<Xi>_wordarray_fold_no_break_0 wordarray_fold_no_break_0_type_def abbreviated_type_defs)
       apply (rule_tac x = ra in exI)
       apply (rule conjI)
        apply (intro exI, assumption)
       apply (rule_tac x = ro in exI)
-      apply (rule conjI)
-       apply (erule u_t_unittE; clarsimp intro!: upd.u_t_unit)
+      apply (rule conjI, simp)
       apply (unfold foldmap_bounds_def)
       apply (erule conjE)+
       apply (case_tac "t5_C.frm_C v' < e")
@@ -1153,6 +1158,423 @@ gets (\<lambda>s. x)
    apply (rule conjI; clarsimp)
    apply (rename_tac j)
    apply (erule_tac x = j in allE; clarsimp)
+  apply (subst min_def)
+  apply (clarsimp simp: not_le)
+  done
+
+lemma \<Xi>_wordarray_map_no_break_0:
+  "\<Xi> ''wordarray_map_no_break_0'' = wordarray_map_no_break_0_type"
+  by (clarsimp simp: \<Xi>_def)
+
+lemma map_dispatch_wp:
+  "\<lbrakk>proc_ctx_wellformed \<Xi>; upd.proc_env_matches_ptrs \<xi>0 \<Xi>;
+    wa_abs_typing_u (UWA (TPrim (Num U32)) len arr) ''WordArray'' [TPrim (Num U32)] (Boxed Writable ptrl) r w \<sigma>;
+    \<sigma> p = option.Some (UAbstract (UWA (TPrim (Num U32)) len arr));
+    upd.uval_typing \<Xi> \<sigma> acc (foldmap_acc_type ''wordarray_map_no_break_0'') ra wa;
+    upd.uval_typing \<Xi> \<sigma> obsv (foldmap_obsv_type ''wordarray_map_no_break_0'') ro {}; wa \<inter> r = {}; p \<notin> w;
+    p \<notin> r; w \<inter> wa = {}; w \<inter> (ra \<union> ro) = {}; wa \<inter> ro = {}; p \<notin> wa; p \<notin> ra; p \<notin> ro; p = ptr_val p';
+    (\<Xi>, [], [option.Some (foldmap_funarg_type ''wordarray_map_no_break_0'')] \<turnstile> 
+    (App f (Var 0)) : (foldmap_funret_type ''wordarray_map_no_break_0''));
+    \<forall>x x' \<sigma> s. val_rel x x' \<longrightarrow>
+      update_sem_init.corres wa_abs_typing_u wa_abs_repr (Generated.state_rel wa_abs_repr) 
+        (App f (Var 0)) (do ret <- dispatch_t8' f_num x'; gets (\<lambda>s. ret) od) 
+        \<xi>0 [x] \<Xi> [option.Some (foldmap_funarg_type ''wordarray_map_no_break_0'')] \<sigma> s\<rbrakk> \<Longrightarrow>
+    \<lbrace>\<lambda>sa. (a', n') = (a, n) \<and> n < e \<and>
+      (\<exists>\<sigma>' res x v. args = t6_C.elem_C_update (\<lambda>_. v) a \<and>
+        \<sigma>' (arr + size_of_num_type U32 * n) = option.Some x \<and> val_rel x v \<and>
+      foldmap_inv upd_wa_mapAccumnb_bod \<xi>0 \<sigma> p frm n f acc obsv (ra \<union> ro) \<sigma>' res sa (t10_C p' (t6_C.acc_C args))) \<and>
+      foldmap_bounds frm to len n e \<and> foldmap_inv_stat obsv (t6_C.obsv_C args)\<rbrace>
+      dispatch_t8' f_num args 
+     \<lbrace>\<lambda>ret sb. (\<exists>\<sigma>' res. 
+        foldmap_inv upd_wa_mapAccumnb_bod \<xi>0 \<sigma> p frm (n + 1) f acc obsv (ra \<union> ro) \<sigma>' res 
+          (heap_w32_update (\<lambda>x a. if a = values_C (heap_WordArray_u32_C sb p') +\<^sub>p uint n 
+            then t7_C.p1_C ret else x a) sb) (t10_C p' (t7_C.p2_C ret))) \<and>
+        foldmap_inv_stat obsv (t6_C.obsv_C args) \<and>
+        foldmap_bounds frm to len (n + 1) e \<and>
+        foldmap_measure (n + 1) to < foldmap_measure n' to \<and>
+        is_valid_WordArray_u32_C sb p' \<and>
+        is_valid_w32 sb (values_C (heap_WordArray_u32_C sb p') +\<^sub>p uint n)\<rbrace>!"
+  apply (subst validNF_def)
+  apply (clarsimp simp: \<Xi>_wordarray_map_no_break_0 wordarray_map_no_break_0_type_def abbreviated_type_defs)
+  apply (rule conjI)
+   apply (subst valid_def)
+   apply (clarsimp simp: foldmap_inv_def)
+   apply (rename_tac sa ret sb \<sigma>' res x v)
+   apply (frule upd_wa_mapAccumnb_bod_preservation'; simp?)
+   apply clarsimp
+   apply (rename_tac racc)
+   apply (erule_tac x = "mk_urecord [x, racc, obsv]" in allE)
+   apply (erule_tac x = args in allE)
+   apply clarsimp
+   apply (erule impE)
+    apply (clarsimp simp: val_rel_simp foldmap_inv_stat_def)
+   apply (erule_tac x = \<sigma>' in allE)
+   apply (erule_tac x = sa in allE)
+   apply (clarsimp simp: corres_def)
+   apply (frule_tac t = "TPrim (Num U32)" in upd_wa_mapAccumnb_bod_preservation; simp?; clarsimp?)
+     apply (subst Int_Un_distrib2; clarsimp)
+     apply (subst (asm) Int_Un_distrib; clarsimp)
+    apply (subst (asm) Int_Un_distrib; clarsimp)
+   apply (rename_tac r' w')
+   apply (erule upd.u_t_recE; clarsimp)
+   apply (erule upd.u_t_r_consE; simp)
+   apply (erule conjE)+
+   apply (drule_tac t = "type_repr _" in sym; clarsimp)
+   apply (erule upd.u_t_r_consE; clarsimp)
+   apply (erule upd.u_t_r_emptyE; clarsimp)
+   apply (rename_tac w' rb wb racc rc wc)
+   apply (erule upd.u_t_p_con_wrE)
+   apply (drule_tac t = "RCon _ _" in sym; clarsimp)
+   apply (frule_tac p = p in valid_ptr_not_in_frame_same; simp?)
+   apply clarsimp
+   apply (frule_tac p = p in readonly_not_in_frame; simp?)
+   apply (subst (asm) insert_ident; clarsimp)
+   apply (rename_tac wb)
+   apply (subgoal_tac "upd.matches_ptrs \<Xi> \<sigma>' [(mk_urecord [x, racc, obsv])]
+      [option.Some (foldmap_funarg_type ''wordarray_map_no_break_0'')] (rc \<union> ro) wc")
+    apply (clarsimp simp: \<Xi>_wordarray_map_no_break_0 wordarray_map_no_break_0_type_def abbreviated_type_defs)
+    apply (erule impE, blast)
+    apply clarsimp
+    apply (erule_tac x = ret in allE)
+    apply (erule_tac x = sb in allE)
+    apply clarsimp
+    apply (drule upd.preservation[where \<tau>s = "[]" and K = "[]", simplified]; simp?)
+    apply clarsimp
+    apply (rename_tac \<sigma>'' res' r' w')
+    apply (erule u_t_rectE; clarsimp)
+    apply (erule u_t_r_contE; clarsimp)
+    apply (erule u_t_r_contE; clarsimp)
+    apply (erule u_t_r_contE; clarsimp)
+    apply (rename_tac x' rd wd racc' r' w')
+    apply (frule_tac v = x' in upd.tprim_no_pointers(1); clarsimp)
+    apply (frule_tac v = x' in upd.tprim_no_pointers(2); clarsimp)
+    apply (clarsimp simp: foldmap_bounds_def)
+    apply (case_tac "frm < to \<and> frm < len"; clarsimp)
+    apply (thin_tac "wa_abs_typing_u _ _ _ _ _ _ _")
+    apply (drule_tac t = U32 and arr = arr and len = len and v' = x' and r' = racc'
+      in upd_wa_mapAccumnb_bod_step; simp?; clarsimp?)
+       apply (drule wa_abs_typing_u_elims(6); simp?)
+      apply (subst Int_Un_distrib2)+
+      apply clarsimp
+      apply (rule conjI)
+       apply (rule disjointI)
+       apply (rename_tac y y')
+       apply (frule_tac p = y and r = ra and w = wa in upd.uval_typing_valid(1)[rotated 1]; simp?)
+       apply clarsimp
+       apply (drule_tac p = y' in readonly_not_in_frame; simp?)
+       apply (drule_tac x = y' and S' = "ra \<union> ro" in orthD2; simp?)
+       apply (drule upd.uval_typing_pointers_noalias)
+       apply (drule_tac x = y' and S = ra and S' = wa in orthD1; simp?)
+      apply (rule conjI)
+       apply (rule disjointI)
+       apply (rename_tac y y')
+       apply (frule_tac p = y and r = ro and w = "{}" in upd.uval_typing_valid(1)[rotated 1]; simp?)
+       apply clarsimp
+       apply (drule_tac p = y' in readonly_not_in_frame; simp?)
+       apply blast
+      apply (drule wa_abs_typing_u_elims(3); clarsimp)
+     apply (drule_tac v = x' in upd.type_repr_uval_repr(1); simp)
+     apply (drule_tac v = racc' in upd.type_repr_uval_repr(1); simp)
+    apply (thin_tac "_ \<in> state_rel")
+    apply (clarsimp simp: state_rel_def heap_rel_def heap_rel_ptr_meta heap_rel_ptr_w32_meta)
+    apply (frule_tac p = p and \<sigma> = \<sigma>' in valid_ptr_not_in_frame_same; simp?)
+    apply (drule_tac p = "arr + 4 * n" and \<sigma> = \<sigma>' in valid_ptr_not_in_frame_same; simp?)
+     apply (drule_tac x = "arr + 4 * n" and S' = wc in orthD1; simp?)
+     apply (drule wa_abs_typing_u_elims(3); clarsimp)
+     apply (rule_tac x = n in exI; clarsimp)
+    apply (frule_tac p = p' in all_heap_rel_ptrD; simp?)
+     apply (clarsimp simp: type_rel_simp wa_abs_repr_def)
+    apply (frule_tac p = "values_C (heap_WordArray_u32_C sb p') +\<^sub>p uint n" and uv = x in all_heap_rel_ptrD; simp?)
+      apply (clarsimp simp: val_rel_simp heap_simp)
+     apply (clarsimp simp: type_rel_simp val_rel_simp)
+    apply (rule conjI)
+     apply (rule_tac x = "\<sigma>''(arr + 4 * n \<mapsto> x')" in exI)
+     apply (rule_tac x = "mk_urecord [UPtr (ptr_val p') (RCon ''WordArray'' [RPrim (Num U32)]), racc']" in exI)
+     apply clarsimp
+     apply (rule conjI)
+      apply (clarsimp simp: val_rel_simp)
+     apply (clarsimp simp: heap_simp is_valid_simp)
+     apply (drule_tac upd_h = "(heap_w32_update 
+      (\<lambda>x a. if a = values_C (heap_WordArray_u32_C sb p') +\<^sub>p uint n then t7_C.p1_C ret else x a) sb)" and
+      uv = x and uv' = x' and x = "values_C (heap_WordArray_u32_C sb p') +\<^sub>p uint n"
+      in all_heap_rel_updE; simp?; clarsimp?)
+        apply (clarsimp simp: val_rel_simp)
+       apply (drule_tac v = x' in upd.type_repr_uval_repr(1); simp add: val_rel_simp)
+      apply (clarsimp simp: val_rel_simp type_rel_simp)
+     apply (drule_tac upd_h = "(heap_w32_update 
+      (\<lambda>x a. if a = values_C (heap_WordArray_u32_C sb p') +\<^sub>p uint n then t7_C.p1_C ret else x a) sb)" and
+      uv = x and uv' = x' and x = "values_C (heap_WordArray_u32_C sb p') +\<^sub>p uint n"
+      in all_heap_rel_updE; simp?; clarsimp?)
+        apply (clarsimp simp: val_rel_simp)
+       apply (drule_tac v = x' in upd.type_repr_uval_repr(1); simp add: val_rel_simp)
+      apply (rule conjI)
+       apply (clarsimp simp: val_rel_simp)
+      apply (cut_tac p = pa and q = "values_C (heap_WordArray_u32_C sb p') +\<^sub>p uint n" in ptr_val_inj)
+      apply clarsimp
+     apply (clarsimp simp: ptr_add_def mult.commute val_rel_simp)
+    apply (clarsimp simp: is_valid_simp)
+    apply (frule_tac a = n and k = to in less_is_non_zero_p1)
+    apply (drule unatSuc2; clarsimp simp: word_less_nat_alt word_le_nat_alt foldmap_measure_def)
+    apply linarith
+  apply (clarsimp simp: \<Xi>_wordarray_map_no_break_0 wordarray_map_no_break_0_type_def abbreviated_type_defs)
+   apply (rule upd.matches_ptrs_some[where r' = "{}" and w' = "{}", simplified])
+    apply (rule upd.u_t_struct; simp?)
+    apply (rule upd.u_t_r_cons1[where r = "{}" and w = "{}", simplified]; simp?)
+      apply (subst (asm) val_rel_word; clarsimp)
+      apply (rule upd.u_t_prim'; clarsimp)
+     apply (rule upd.u_t_r_cons1[where r' = ro and w' = "{}", simplified]; simp?)
+      apply (drule_tac u = obsv in upd.uval_typing_frame(1); simp?)
+       apply blast
+      apply (rule upd.u_t_r_cons1[where r' = "{}" and w' = "{}", simplified]; simp?)
+       apply (rule upd.u_t_r_empty)
+      apply (drule_tac v = obsv in upd.type_repr_uval_repr(1); simp)
+     apply (rule disjointI)
+     apply (frule_tac p = y and r = ro in upd.uval_typing_valid(1)[where w = "{}", simplified]; simp?)
+     apply clarsimp
+     apply (drule_tac p = y in readonly_not_in_frame; simp?)
+     apply (drule_tac x = y and S' = ro in orthD2; simp?)
+     apply (drule_tac x = y and S' = "ra \<union> ro" in orthD2; simp?)
+    apply (subst (asm) val_rel_word; clarsimp)
+   apply (rule upd.matches_ptrs_empty[where \<tau>s = "[]", simplified])
+  apply (subst no_fail_def)
+  apply clarsimp
+  apply (clarsimp simp: foldmap_inv_def)
+  apply (rename_tac sa \<sigma>' res x v)
+  apply (frule upd_wa_mapAccumnb_bod_preservation'; simp?)
+  apply clarsimp
+  apply (rename_tac racc)
+  apply (erule_tac x = "mk_urecord [x, racc, obsv]" in allE)
+  apply (erule_tac x = args in allE)
+  apply clarsimp
+  apply (erule impE)
+   apply (clarsimp simp: val_rel_simp foldmap_inv_stat_def)
+  apply (erule_tac x = \<sigma>' in allE)
+  apply (erule_tac x = sa in allE)
+  apply (clarsimp simp: corres_def)
+  apply (frule_tac t = "TPrim (Num U32)" in upd_wa_mapAccumnb_bod_preservation; simp?; clarsimp?)
+    apply (subst Int_Un_distrib2; clarsimp)
+    apply (subst (asm) Int_Un_distrib; clarsimp)
+   apply (subst (asm) Int_Un_distrib; clarsimp)
+  apply (rename_tac r' w')
+  apply (erule upd.u_t_recE; clarsimp)
+  apply (erule upd.u_t_r_consE; simp)
+  apply (erule conjE)+
+  apply (drule_tac t = "type_repr _" in sym; clarsimp)
+  apply (erule upd.u_t_r_consE; clarsimp)
+  apply (erule upd.u_t_r_emptyE; clarsimp)
+  apply (rename_tac w' rb wb racc rc wc)
+  apply (erule upd.u_t_p_con_wrE)
+  apply (drule_tac t = "RCon _ _" in sym; clarsimp)
+  apply (frule_tac p = p in readonly_not_in_frame; simp?)
+  apply (subst (asm) insert_ident; clarsimp)
+  apply (erule_tac x = "rc \<union> ro" in allE)
+  apply (erule_tac x = wc in allE)
+  apply (rotate_tac -1)
+  apply (erule notE)
+  apply (rule upd.matches_ptrs_some[where r' = "{}" and w' = "{}", simplified])
+   apply (rule upd.u_t_struct; simp?)
+   apply (rule upd.u_t_r_cons1[where r = "{}" and w = "{}", simplified]; simp?)
+     apply (subst (asm) val_rel_word; clarsimp)
+     apply (rule upd.u_t_prim'; clarsimp)
+    apply (rule upd.u_t_r_cons1[where r' = ro and w' = "{}", simplified]; simp?)
+     apply (drule_tac u = obsv in upd.uval_typing_frame(1); simp?)
+      apply blast
+     apply (rule upd.u_t_r_cons1[where r' = "{}" and w' = "{}", simplified]; simp?)
+      apply (rule upd.u_t_r_empty)
+     apply (drule_tac v = obsv in upd.type_repr_uval_repr(1); simp)
+    apply (rule disjointI)
+    apply (frule_tac p = y and r = ro in upd.uval_typing_valid(1)[where w = "{}", simplified]; simp?)
+    apply clarsimp
+    apply (drule_tac p = y in readonly_not_in_frame; simp?)
+    apply (drule_tac x = y and S' = ro in orthD2; simp?)
+    apply (drule_tac x = y and S' = "ra \<union> ro" in orthD2; simp?)
+   apply (subst (asm) val_rel_word; clarsimp)
+  apply (rule upd.matches_ptrs_empty[where \<tau>s = "[]", simplified])
+  done
+
+lemma upd_C_wordarray_map_no_break_corres':
+  "\<lbrakk>upd.proc_env_matches_ptrs \<xi>0 \<Xi>; i < length \<gamma>; val_rel (\<gamma> ! i) v';
+    \<Gamma>' ! i = option.Some (prod.fst (prod.snd (\<Xi> ''wordarray_map_no_break_0'')));
+    \<gamma> ! i = URecord fs; f = prod.fst (fs ! 3); obsv = prod.fst (fs ! 5);
+    upd.uval_typing \<Xi> \<sigma> obsv (foldmap_obsv_type ''wordarray_map_no_break_0'') ro {};
+    (\<Xi>, [], [option.Some (foldmap_funarg_type ''wordarray_map_no_break_0'')] \<turnstile> 
+    (App (uvalfun_to_exprfun f) (Var 0)) : (foldmap_funret_type ''wordarray_map_no_break_0''));
+    \<forall>x x' \<sigma> s. val_rel x x' \<longrightarrow> update_sem_init.corres wa_abs_typing_u wa_abs_repr (Generated.state_rel wa_abs_repr) 
+      (App (uvalfun_to_exprfun f) (Var 0)) (do ret <- dispatch_t8' (t9_C.f_C v') x'; gets (\<lambda>s. ret) od) 
+      \<xi>0 [x] \<Xi> [option.Some (foldmap_funarg_type ''wordarray_map_no_break_0'')] \<sigma> s\<rbrakk>
+    \<Longrightarrow> update_sem_init.corres wa_abs_typing_u wa_abs_repr (Generated.state_rel wa_abs_repr)
+         (App (AFun ''wordarray_map_no_break_0'' []) (Var i)) (do x <- main_pp_inferred.wordarray_map_no_break_0' v';
+gets (\<lambda>s. x)
+                                                                od)
+         \<xi>1 \<gamma> \<Xi>  \<Gamma>' \<sigma> s"
+  apply (rule absfun_corres; simp)
+  apply (clarsimp simp: abs_fun_rel_def'; rename_tac r w)
+  apply (thin_tac "\<Gamma>' ! i = _")
+  apply (subst \<xi>1.simps)
+  apply (subst (asm) val_rel_simp; clarsimp)
+  apply (subst (asm) val_rel_ptr_def; clarsimp)
+  apply (subst (asm) val_rel_fun_tag)
+  apply (subst (asm) val_rel_word)
+  apply (subst (asm) val_rel_word)
+  apply (clarsimp simp: upd_wa_mapAccumnb_def wordarray_map_no_break_0'_def)
+  apply (rename_tac pwa_rep frm_rep to_rep f_rep acc a_rep o_rep wa_rep)
+  apply (erule upd.u_t_recE; clarsimp)
+  apply (clarsimp simp: \<Xi>_wordarray_map_no_break_0 wordarray_map_no_break_0_type_def abbreviated_type_defs)
+  apply (erule upd.u_t_r_consE; clarsimp)
+  apply (rename_tac r w r' w')
+  apply (erule upd.u_t_p_absE; clarsimp)
+  apply (rename_tac w)
+  apply (frule wa_abs_typing_u_elims(1); clarsimp)
+  apply (erule upd.u_t_r_consE; simp)
+  apply (erule upd.u_t_r_consE; simp)
+  apply (erule conjE)+
+  apply (drule_tac t = "type_repr _" in sym)+
+  apply clarsimp
+  apply (erule upd.u_t_primE)+
+  apply (drule_tac t = "lit_type _" in sym)+
+  apply clarsimp
+  apply (erule upd.u_t_r_consE; clarsimp)+
+  apply (erule upd.u_t_r_emptyE; clarsimp)
+  apply (frule upd.tfun_no_pointers(1))
+  apply (frule upd.tfun_no_pointers(2))
+  apply clarsimp
+  apply (rename_tac acc ra wa ro' wo)
+  apply (drule_tac x = obsv in upd.uval_typing_unique_ptrs(1); simp?)
+  apply (subst unknown_bind_ignore)+
+  apply (clarsimp simp: join_guards) 
+  apply wp
+      apply (clarsimp simp: unknown_bind_ignore split: prod.split)
+       apply (rename_tac var e)
+       apply (rule_tac M = "\<lambda>((_, i), _). foldmap_measure i (t9_C.to_C v')" and 
+      I = "\<lambda>(a, b) s. (\<exists>\<sigma>' res. foldmap_inv upd_wa_mapAccumnb_bod \<xi>0 \<sigma> (ptr_val (t9_C.arr_C v'))
+          (t9_C.frm_C v') b (uvalfun_to_exprfun f) acc obsv (ra \<union> ro) \<sigma>' res s (t10_C (t9_C.arr_C v') (t6_C.acc_C a))) \<and>
+          foldmap_inv_stat obsv (t6_C.obsv_C a) \<and>
+          foldmap_bounds (t9_C.frm_C v') (t9_C.to_C v') len b e" in whileLoop_add_invI; simp?)
+       apply (wp; clarsimp simp: unknown_bind_ignore split: prod.splits)
+           apply (rename_tac sa a n args a' n')
+           apply (clarsimp simp: conj_left_commute[of "is_valid_w32 _ _", simplified])
+           apply (clarsimp simp: conj_commute[of "is_valid_w32 _ _", simplified])
+           apply (rule_tac a = a and wa = wa and ra = ra and ro = ro and w = w and r = r and
+              ptrl = undefined in map_dispatch_wp; simp?)
+              apply (clarsimp simp: \<Xi>_wordarray_map_no_break_0 wordarray_map_no_break_0_type_def abbreviated_type_defs)+
+          apply wp
+         apply wp
+        apply clarsimp
+        apply (rename_tac args j \<sigma>' res)
+        apply (clarsimp simp: foldmap_inv_def foldmap_bounds_def)
+        apply (drule upd_wa_mapAccumnb_bod_preservation; simp?; clarsimp?)
+          apply (subst Int_Un_distrib2; clarsimp)
+          apply (cut_tac A = w and B = ra and C = ro in Int_Un_distrib; clarsimp)
+         apply (cut_tac A = w and B = ra and C = ro in Int_Un_distrib; clarsimp)
+        apply (frule_tac p = "ptr_val (t9_C.arr_C v')" in valid_ptr_not_in_frame_same; simp?)
+        apply (thin_tac "_ \<in> state_rel")
+        apply (frule_tac upd_wa_mapAccumnb_bod_preservation'; simp?)
+        apply clarsimp
+        apply (erule upd.u_t_recE; clarsimp)
+        apply (erule upd.u_t_r_consE; simp)
+        apply (erule conjE)+
+        apply (drule_tac t = "type_repr _" in sym; clarsimp)
+        apply (erule upd.u_t_p_con_wrE)
+        apply (drule_tac t = "RCon _ _" in sym; clarsimp)
+        apply (thin_tac "wa_abs_typing_u _ _ _ _ _ _ _")
+        apply (drule wa_abs_typing_u_elims(5))
+        apply (erule_tac x = j in allE; clarsimp)
+        apply (clarsimp simp: state_rel_def heap_rel_def heap_rel_ptr_meta heap_rel_ptr_w32_meta)
+        apply (frule_tac p = "t9_C.arr_C v'" in all_heap_rel_ptrD; simp?)
+         apply (clarsimp simp: type_rel_simp wa_abs_repr_def)
+        apply (rotate_tac -2)
+         apply (frule_tac p = "Ptr(arr + 4 * j)" in all_heap_rel_ptrD; simp?)
+         apply (clarsimp simp: type_rel_simp)
+        apply (rule conjI)
+         apply (rule_tac x = \<sigma>' in exI)
+         apply (rule_tac x = "mk_urecord [UPtr (ptr_val (t9_C.arr_C v'))
+          (RCon ''WordArray'' [RPrim (Num U32)]), racc]" in exI)
+         apply (rule_tac x = "UPrim x" in exI)
+         apply (rule_tac x = "heap_w32 s (PTR(32 word) (arr + 4 * j))" in exI)
+         apply (clarsimp simp: val_rel_WordArray_u32_C_def ptr_add_def heap_simp mult.commute)
+        apply (clarsimp simp: val_rel_WordArray_u32_C_def ptr_add_def is_valid_simp heap_simp mult.commute)
+       apply (rule conjI)
+        apply (drule_tac v = acc in upd.type_repr_uval_repr(1); simp)
+       apply (rule conjI)
+        apply (drule_tac v = obsv in upd.type_repr_uval_repr(1); simp)
+       apply (rule conjI)
+        apply (drule wa_abs_typing_u_elims(5); simp)
+       apply (rule conjI)
+        apply (erule u_t_funafuntE; clarsimp)
+       apply (rule_tac x = \<sigma>' in exI)
+       apply (rule_tac x = res in exI)
+       apply (clarsimp simp: foldmap_inv_def)
+       apply (rule conjI)
+        apply (rule_tac x = "foldmap_acc_type ''wordarray_map_no_break_0''" in exI)
+        apply (rule_tac x = "foldmap_obsv_type ''wordarray_map_no_break_0''" in exI)
+        apply (rule_tac x = "''elem''" in exI)
+        apply (rule_tac x = "''acc''" in exI)
+        apply (rule_tac x = "''obsv''" in exI)
+        apply (rule_tac x = "''p1''" in exI)
+        apply (rule_tac x = "''p2''" in exI)
+        apply (rule_tac x = ra in exI)
+        apply (clarsimp simp: \<Xi>_wordarray_map_no_break_0 wordarray_map_no_break_0_type_def abbreviated_type_defs)
+        apply (rule conjI)
+         apply (intro exI, assumption)
+        apply (rule_tac x = ro in exI)
+        apply clarsimp
+        apply (rename_tac j \<sigma>' res)
+        apply (unfold foldmap_bounds_def)
+        apply (erule conjE)+
+        apply (case_tac "t9_C.frm_C v' < e")
+         apply (erule impE, assumption)
+         apply (thin_tac "_ \<longrightarrow> _")
+         apply clarsimp
+         apply (case_tac "j < t9_C.to_C v'"; clarsimp)
+         apply (rule upd_wa_mapAccumnb_bod_to_geq_len; simp?)
+        apply (erule impE, assumption)
+        apply (thin_tac "_ \<longrightarrow> _")
+        apply clarsimp
+        apply (erule upd_wa_mapAccumnb_bod.elims; clarsimp)
+        apply (case_tac "t9_C.frm_C v' < t9_C.to_C v'"; subst upd_wa_mapAccumnb_bod.simps; clarsimp)
+       apply (clarsimp simp: val_rel_simp)
+      apply wp
+     apply wp
+    apply (rule validNF_select_UNIV)
+   apply (rule validNF_select_UNIV)
+  apply (clarsimp simp: foldmap_inv_stat_def)
+  apply (clarsimp simp: order.strict_implies_order)
+  apply (clarsimp simp: foldmap_inv_def state_rel_def heap_rel_def heap_rel_ptr_meta)
+  apply (frule_tac p = "t9_C.arr_C v'" in all_heap_rel_ptrD; simp?)
+   apply (clarsimp simp: type_rel_simp wa_abs_repr_def)
+  apply (clarsimp simp: is_valid_simp val_rel_WordArray_u32_C_def heap_simp)
+  apply (rule conjI; clarsimp)
+   apply (rule conjI)
+    apply (rule_tac x = \<sigma> in exI)
+    apply (rule_tac x = "mk_urecord [UPtr (ptr_val (t9_C.arr_C v'))
+      (RCon ''WordArray'' [RPrim (Num U32)]), acc]" in exI)
+    apply (subst upd_wa_mapAccumnb_bod.simps; clarsimp)
+    apply (rule conjI)
+     apply (drule wa_abs_typing_u_elims(5); clarsimp)
+     apply (rename_tac j)
+     apply (erule_tac x = j in allE; clarsimp)
+    apply (rule conjI)
+     apply (drule wa_abs_typing_u_elims(3); clarsimp)
+    apply (rule conjI)
+     apply (clarsimp simp: val_rel_simp)
+    apply (rule conjI; clarsimp)
+   apply (subst min_def)
+   apply (subst (asm) not_le[symmetric])+
+   apply (subst if_not_P; simp?)
+  apply (rule conjI)
+   apply (rule_tac x = \<sigma> in exI)
+   apply (rule_tac x = "mk_urecord [UPtr (ptr_val (t9_C.arr_C v'))
+      (RCon ''WordArray'' [RPrim (Num U32)]), acc]" in exI)
+   apply (subst upd_wa_mapAccumnb_bod.simps; clarsimp)
+   apply (rule conjI)
+    apply (drule wa_abs_typing_u_elims(5); clarsimp)
+    apply (rename_tac j)
+    apply (erule_tac x = j in allE; clarsimp)
+   apply (rule conjI)
+    apply (drule wa_abs_typing_u_elims(3); clarsimp)
+   apply (rule conjI)
+    apply (clarsimp simp: val_rel_simp)
+   apply (rule conjI; clarsimp)
   apply (subst min_def)
   apply (clarsimp simp: not_le)
   done
